Sodium.lean
@@ -1,1 +1,1 @@
-import «Sodium».Crypto.Spec
+import «Sodium».Crypto.Monad
